theories/logrel/logrel.v
@@ -3,7 +3,53 @@ From machine_program_logic.program_logic Require Import weakestpre.
 From HypVeri.lang Require Import lang.
 From HypVeri Require Import big_sepFM machine_extra.
 From HypVeri.algebra Require Import base base_extra mem mailbox trans.
+From HypVeri.logrel Require Import big_sepSS.
 Import uPred.
+
+
+Section slice_trans.
+  Context `{hypconst:HypervisorConstants}.
+  Context `{vmG: !gen_VMG Σ}.
+  Context (Φ : (gmap Addr transaction) -> VMID -> VMID -> iProp Σ).
+
+  Definition trans_preserve_slice i j (trans trans': (gmap Addr transaction)):=
+    filter (λ kv, kv.2.1.1.1.1 = i ∧ kv.2.1.1.1.2 = j) trans
+                        = filter (λ kv, kv.2.1.1.1.1 = i ∧ kv.2.1.1.1.2 = j) trans'.
+
+  Class SliceTransWf :=
+    {
+      slice_trans_valid : ∀ i j trans trans',
+        trans_preserve_slice i j trans trans'-> (Φ trans i j ⊣⊢ Φ trans' i j)
+    }.
+
+
+End slice_trans.
+
+Global Arguments SliceTransWf {_} {_} _.
+Global Arguments slice_trans_valid {_} {_} _ {_} {_} {_} {_} {_} _.
+Global Hint Mode SliceTransWf + + ! : typeclass_instances.
+
+Section slice_rxs.
+  Context `{hypconst:HypervisorConstants}.
+  Context `{vmG: !gen_VMG Σ}.
+  Context (Φ :VMID -> option (Word * VMID)-> VMID -> iProp Σ).
+
+  Class SliceRxsWf :=
+    {
+      slice_rxs_empty : ∀ i j, Φ i None j ⊣⊢ True;
+      slice_rxs_sym : ∀ i os k k',
+        (match os with
+         | None => True
+         | Some (_,j) => j ≠ V0 ->  Φ i os k ⊣⊢ Φ i os k'
+         end);
+    }.
+
+End slice_rxs.
+
+Global Arguments SliceRxsWf {_} {_} _.
+Global Arguments slice_rxs_empty {_} {_} _ {_} _ _.
+Global Arguments slice_rxs_sym {_} {_} _ {_} {_} {_} _ _.
+Global Hint Mode SliceRxsWf + + ! : typeclass_instances.
 
 (**  unary logical relation **)
 Section logrel.
@@ -11,6 +57,7 @@ Section logrel.
   Context `{hypparams:!HypervisorParameters}.
   Context `{vmG: !gen_VMG Σ}.
 
+  Definition set_of_vmids : gset VMID := (list_to_set list_of_vmids).
   Definition lift_option_gmap`{Countable K} {V: Type} (m: gmap K V) := (λ v, Some v) <$> m.
   Definition pages_in_trans (trans: gmap Word transaction) : gset PID :=
     pages_in_trans' (lift_option_gmap trans).
@@ -108,16 +155,16 @@ Section logrel.
   Definition rx_state_get (i:VMID) (rxs: gmap VMID (option (Word*VMID))) :iProp Σ:=
     ∀ rs, ⌜rxs !! i = Some rs⌝ -∗ RX_state@i := rs.
 
-  (* [TODO] *)
-  Definition return_reg_rx i (rs : option (Word * VMID)) (rxs :gmap VMID (option(Word*VMID))): iProp Σ:=
-    ((R0 @@ V0 ->r encode_hvc_func(Yield) ∨
-      R0 @@ V0 ->r encode_hvc_func(Wait) ∗ ⌜rs = None⌝)
-     ∗ rx_states_global (delete i rxs)
-     ∗ R1 @@ V0 ->r encode_vmid(i) ∗ ∃ r2, R2 @@ V0 ->r r2) ∨
-    (R0 @@ V0 ->r encode_hvc_func(Send)
-      ∗ ∃ l j, RX_state{1/2}@j := Some(l,i) ∗ (∃ p_rx, RX@ j := p_rx ∗ ∃ mem_rx, memory_page p_rx mem_rx)
-      ∗ rx_states_global (<[j:=Some(l,i)]>(delete i rxs)) ∗ ⌜rxs !! j = Some None⌝
-      ∗ (∃r1, R1 @@ V0 ->r r1 ∗ ⌜decode_vmid r1 = Some j⌝) ∗  R2 @@ V0 ->r l).
+  (* (* [TODO] *) *)
+  (* Definition return_reg_rx i (rs : option (Word * VMID)) (rxs :gmap VMID (option(Word*VMID))): iProp Σ:= *)
+  (*   ((R0 @@ V0 ->r encode_hvc_func(Yield) ∨ *)
+  (*     R0 @@ V0 ->r encode_hvc_func(Wait) ∗ ⌜rs = None⌝) *)
+  (*    ∗ rx_states_global (delete i rxs) *)
+  (*    ∗ R1 @@ V0 ->r encode_vmid(i) ∗ ∃ r2, R2 @@ V0 ->r r2) ∨ *)
+  (*   (R0 @@ V0 ->r encode_hvc_func(Send) *)
+  (*     ∗ ∃ l j, RX_state{1/2}@j := Some(l,i) ∗ (∃ p_rx, RX@ j := p_rx ∗ ∃ mem_rx, memory_page p_rx mem_rx) *)
+  (*     ∗ rx_states_global (<[j:=Some(l,i)]>(delete i rxs)) ∗ ⌜rxs !! j = Some None⌝ *)
+  (*     ∗ (∃r1, R1 @@ V0 ->r r1 ∗ ⌜decode_vmid r1 = Some j⌝) ∗  R2 @@ V0 ->r l). *)
 
   Definition only (trans: gmap Word transaction) := (filter (λ (kv :Word*transaction), (kv.2.1.1.1.1 = i ∨ kv.2.1.1.1.2 = i)) trans).
 
@@ -141,81 +188,202 @@ Section logrel.
   (*   dom (filter (λ kv, (kv.2.1.1.1.2 = i ∧ kv.2.2 = true)) trans') *)
   (*   ⊆ dom (filter (λ kv, (kv.2.1.1.1.2 = i ∧ kv.2.2 = true)) trans). *)
 
-  Definition vmprop_zero_pre (Ψ: (gmap Word transaction) -d> iPropO Σ) : (gmap Word transaction) -d> (gmap VMID (option(Word*VMID))) -d> iPropO Σ :=
-    λ trans rxs, (∃ trans' rs',
+(* Section vmprop. *)
+(*   Context `{HypervisorConstants}. *)
+(*   Context `{!HypervisorParameters}. *)
+(*   Context `{vmG: !gen_VMG Σ}. *)
+  (* Context (i : VMID). *)
+  Context (Φ_t : (gmap Addr transaction) -> VMID -> VMID -> iProp Σ).
+  Context (Φ_r : VMID -> option (Word * VMID)-> VMID -> iProp Σ).
+
+  Definition rx_states_transferred (rxs: gmap VMID (option (Word*VMID))) : iProp Σ :=
+    [∗ map]i ↦ os ∈ rxs, match os with
+                           | None => True
+                           | Some s => Φ_r i os V0
+                          end.
+
+  Definition rx_states_owned (rxs: gmap VMID (option (Word*VMID))) : iProp Σ :=
+    [∗ map]i ↦ os ∈ rxs, match os with
+                           | None => True
+                           | Some s => if bool_decide (s.2 = V0) then Φ_r i os i else True
+                          end.
+
+  Definition return_reg_rx i (rs : option (Word * VMID)) (rxs :gmap VMID (option(Word*VMID))): iProp Σ:=
+    ((R0 @@ V0 ->r encode_hvc_func(Yield) ∨
+      R0 @@ V0 ->r encode_hvc_func(Wait) ∗ ⌜rs = None⌝)
+     ∗ rx_states_global (delete i rxs)
+     ∗ R1 @@ V0 ->r encode_vmid(i) ∗ ∃ r2, R2 @@ V0 ->r r2) ∨
+    (R0 @@ V0 ->r encode_hvc_func(Send)
+      ∗ ∃ l j, Φ_r j (Some (l,i)) V0
+      ∗ rx_states_global (<[j:=Some(l,i)]>(delete i rxs)) ∗ ⌜rxs !! j = Some None⌝
+      ∗ (∃r1, R1 @@ V0 ->r r1 ∗ ⌜decode_vmid r1 = Some j⌝) ∗  R2 @@ V0 ->r l).
+
+  Definition vmprop_zero_pre (Ψ: (gmap Word transaction) -d> iPropO Σ) : (gmap Word transaction) -d> (gmap VMID (option(Word * VMID))) -d> iPropO Σ :=
+    λ trans rxs, (∃ (trans' :gmap Word transaction) rs',
                      let trans_ret := (only trans') ∪ (except trans) in
                            ⌜dom (only trans') ## dom (except trans)⌝ ∗
                            ⌜∀ x, x ≠ i -> trans_rel_secondary x trans trans_ret⌝ ∗
-                           (* transaction and pagetable entries *)
-                           transaction_hpool_global_transferred trans_ret ∗
-                           transaction_pagetable_entries_transferred i trans_ret ∗
-                           retrievable_transaction_transferred i trans_ret ∗
-                           (* memory *)
-                           (∃ mem_trans, memory_pages (transferred_memory_pages trans_ret) mem_trans) ∗
-                           (RX_state@i:= rs') ∗ (∃p_rx, RX@i := p_rx ∗ (∃ mem_rx, memory_page p_rx mem_rx)) ∗
+                           transaction_hpool_global_transferred (trans_ret) ∗
+                           big_sepSS_singleton set_of_vmids i (Φ_t trans_ret) ∗
+                           rx_state_match i rs' ∗ Φ_r i rs' V0 ∗
                            return_reg_rx i rs' rxs ∗
                            VMProp i (Ψ trans_ret) (1/2)%Qp)%I.
 
-  Definition vmprop_unknown_pre (Φ: (gmap Word transaction) -d> iPropO Σ) : (gmap Word transaction) -d> iPropO Σ :=
+  Definition vmprop_unknown_pre
+    (Ψ :(gmap Word transaction) -d> iPropO Σ) : (gmap Word transaction) -d> iPropO Σ :=
    λ trans, (∃ (trans' : gmap Word transaction) (rxs : gmap VMID (option(Word * VMID))),
                ⌜trans_rel_secondary i trans trans'⌝ ∗
                (* transaction and pagetable entries *)
                transaction_hpool_global_transferred trans' ∗
-               transaction_pagetable_entries_transferred i trans' ∗
-               retrievable_transaction_transferred i trans' ∗
-               (* memory *)
-               (∃ mem_trans, memory_pages (transferred_memory_pages trans') mem_trans) ∗
+               big_sepSS_singleton set_of_vmids i (Φ_t trans') ∗
                (∃ r0, R0 @@ V0 ->r r0 ∗ ⌜decode_hvc_func r0 = Some Run⌝) ∗ (∃ r1, R1 @@ V0 ->r r1 ∗ ⌜decode_vmid r1 = Some i⌝)∗ (∃ r2, R2 @@ V0 ->r r2) ∗
-               (rx_state_get i rxs ∗ (∃p_rx, RX@i := p_rx ∗ (∃ mem_rx, memory_page p_rx mem_rx))) ∗
+               (∀ rs : option (Addr * VMID), ⌜rxs !! i = Some rs⌝ -∗ rx_state_match i rs ∗ Φ_r i rs i) ∗
                (* rx pages for all other VMs *)
-               rx_states_global (delete i rxs) ∗ ⌜is_total_gmap rxs⌝ ∗
+               (rx_states_global (delete i rxs)) ∗ ⌜is_total_gmap rxs⌝ ∗
                (* if i yielding, we give following resources back to pvm *)
-               VMProp V0 (vmprop_zero_pre Φ trans' rxs) (1/2)%Qp)%I.
+               VMProp V0 (vmprop_zero_pre Ψ trans' rxs) (1/2)%Qp)%I.
 
   Local Instance vmprop_unknown_pre_contractive : Contractive (vmprop_unknown_pre).
   Proof.
     rewrite /vmprop_unknown_pre => n vmprop_unknown vmprop_unknown' Hvmprop_unknown trans /=.
-    do 15 f_equiv.
+    do 13 f_equiv.
     rewrite /VMProp /=.
     do 6 f_equiv.
     f_contractive.
     rewrite /vmprop_zero_pre.
-    do 12 f_equiv.
+    do 10 f_equiv.
     rewrite /VMProp.
     repeat f_equiv.
-    (* apply Hvmprop_unknown. *)
   Qed.
 
-  Definition vmprop_unknown := fixpoint (vmprop_unknown_pre).
+  Definition vmprop_unknown:= fixpoint (vmprop_unknown_pre).
 
   Definition vmprop_zero := vmprop_zero_pre vmprop_unknown.
 
-  Lemma vmprop_unknown_eq trans : vmprop_unknown trans ⊣⊢
+  Lemma vmprop_unknown_eq trans: vmprop_unknown trans ⊣⊢
     (∃ (trans' : gmap Word transaction) (rxs : gmap VMID (option(Word * VMID))),
                ⌜trans_rel_secondary i trans trans'⌝ ∗
                (* transaction and pagetable entries *)
                transaction_hpool_global_transferred trans' ∗
-               transaction_pagetable_entries_transferred i trans' ∗
-               retrievable_transaction_transferred i trans' ∗
-               (* memory *)
-               (∃ mem_trans, memory_pages (transferred_memory_pages trans') mem_trans) ∗
+               big_sepSS_singleton set_of_vmids i (Φ_t trans') ∗
                (∃ r0, R0 @@ V0 ->r r0 ∗ ⌜decode_hvc_func r0 = Some Run⌝) ∗ (∃ r1, R1 @@ V0 ->r r1 ∗ ⌜decode_vmid r1 = Some i⌝)∗ (∃ r2, R2 @@ V0 ->r r2) ∗
-               (rx_state_get i rxs ∗ (∃p_rx, RX@i := p_rx ∗ (∃ mem_rx, memory_page p_rx mem_rx))) ∗
+               (∀ rs : option (Addr * VMID), ⌜rxs !! i = Some rs⌝ -∗ rx_state_match i rs ∗ Φ_r i rs i) ∗
                (* rx pages for all other VMs *)
-               rx_states_global (delete i rxs) ∗ ⌜is_total_gmap rxs⌝ ∗
+               (rx_states_global (delete i rxs)) ∗ ⌜is_total_gmap rxs⌝ ∗
                (* if i yielding, we give following resources back to pvm *)
-               VMProp V0 (vmprop_zero trans' rxs) (1/2)%Qp)%I.
-    Proof.
-      rewrite /vmprop_unknown.
-      apply (fixpoint_unfold vmprop_unknown_pre).
-    Qed.
+          VMProp V0 (vmprop_zero trans' rxs) (1/2)%Qp)%I.
+  Proof.
+    rewrite /vmprop_unknown.
+    apply (fixpoint_unfold vmprop_unknown_pre).
+  Qed.
 
-  Program Definition interp_access p_tx p_rx ps_acc trans: iPropO Σ:=
+  (* Definition vmprop_zero_pre (Ψ: (gmap Word transaction) -d> iPropO Σ) : (gmap Word transaction) -d> (gmap VMID (option(Word*VMID))) -d> iPropO Σ := *)
+  (*   λ trans rxs, (∃ trans' rs', *)
+  (*                    let trans_ret := (only trans') ∪ (except trans) in *)
+  (*                          ⌜dom (only trans') ## dom (except trans)⌝ ∗ *)
+  (*                          ⌜∀ x, x ≠ i -> trans_rel_secondary x trans trans_ret⌝ ∗ *)
+  (*                          (* transaction and pagetable entries *) *)
+  (*                          transaction_hpool_global_transferred trans_ret ∗ *)
+  (*                          transaction_pagetable_entries_transferred i trans_ret ∗ *)
+  (*                          retrievable_transaction_transferred i trans_ret ∗ *)
+  (*                          (* memory *) *)
+  (*                          (∃ mem_trans, memory_pages (transferred_memory_pages trans_ret) mem_trans) ∗ *)
+  (*                          (RX_state@i:= rs') ∗ (∃p_rx, RX@i := p_rx ∗ (∃ mem_rx, memory_page p_rx mem_rx)) ∗ *)
+  (*                          return_reg_rx i rs' rxs ∗ *)
+  (*                          VMProp i (Ψ trans_ret) (1/2)%Qp)%I. *)
+
+  (* Definition vmprop_unknown_pre (Φ: (gmap Word transaction) -d> iPropO Σ) : (gmap Word transaction) -d> iPropO Σ := *)
+  (*  λ trans, (∃ (trans' : gmap Word transaction) (rxs : gmap VMID (option(Word * VMID))), *)
+  (*              ⌜trans_rel_secondary i trans trans'⌝ ∗ *)
+  (*              (* transaction and pagetable entries *) *)
+  (*              transaction_hpool_global_transferred trans' ∗ *)
+  (*              transaction_pagetable_entries_transferred i trans' ∗ *)
+  (*              retrievable_transaction_transferred i trans' ∗ *)
+  (*              (* memory *) *)
+  (*              (∃ mem_trans, memory_pages (transferred_memory_pages trans') mem_trans) ∗ *)
+  (*              (∃ r0, R0 @@ V0 ->r r0 ∗ ⌜decode_hvc_func r0 = Some Run⌝) ∗ (∃ r1, R1 @@ V0 ->r r1 ∗ ⌜decode_vmid r1 = Some i⌝)∗ (∃ r2, R2 @@ V0 ->r r2) ∗ *)
+  (*              (rx_state_get i rxs ∗ (∃p_rx, RX@i := p_rx ∗ (∃ mem_rx, memory_page p_rx mem_rx))) ∗ *)
+  (*              (* rx pages for all other VMs *) *)
+  (*              rx_states_global (delete i rxs) ∗ ⌜is_total_gmap rxs⌝ ∗ *)
+  (*              (* if i yielding, we give following resources back to pvm *) *)
+  (*              VMProp V0 (vmprop_zero_pre Φ trans' rxs) (1/2)%Qp)%I. *)
+
+  (* Local Instance vmprop_unknown_pre_contractive : Contractive (vmprop_unknown_pre). *)
+  (* Proof. *)
+  (*   rewrite /vmprop_unknown_pre => n vmprop_unknown vmprop_unknown' Hvmprop_unknown trans /=. *)
+  (*   do 15 f_equiv. *)
+  (*   rewrite /VMProp /=. *)
+  (*   do 6 f_equiv. *)
+  (*   f_contractive. *)
+  (*   rewrite /vmprop_zero_pre. *)
+  (*   do 12 f_equiv. *)
+  (*   rewrite /VMProp. *)
+  (*   repeat f_equiv. *)
+  (*   (* apply Hvmprop_unknown. *) *)
+  (* Qed. *)
+
+  (* Definition vmprop_unknown := fixpoint (vmprop_unknown_pre). *)
+
+  (* Definition vmprop_zero := vmprop_zero_pre vmprop_unknown. *)
+
+  (* Lemma vmprop_unknown_eq trans : vmprop_unknown trans ⊣⊢ *)
+  (*   (∃ (trans' : gmap Word transaction) (rxs : gmap VMID (option(Word * VMID))), *)
+  (*              ⌜trans_rel_secondary i trans trans'⌝ ∗ *)
+  (*              (* transaction and pagetable entries *) *)
+  (*              transaction_hpool_global_transferred trans' ∗ *)
+  (*              transaction_pagetable_entries_transferred i trans' ∗ *)
+  (*              retrievable_transaction_transferred i trans' ∗ *)
+  (*              (* memory *) *)
+  (*              (∃ mem_trans, memory_pages (transferred_memory_pages trans') mem_trans) ∗ *)
+  (*              (∃ r0, R0 @@ V0 ->r r0 ∗ ⌜decode_hvc_func r0 = Some Run⌝) ∗ (∃ r1, R1 @@ V0 ->r r1 ∗ ⌜decode_vmid r1 = Some i⌝)∗ (∃ r2, R2 @@ V0 ->r r2) ∗ *)
+  (*              (rx_state_get i rxs ∗ (∃p_rx, RX@i := p_rx ∗ (∃ mem_rx, memory_page p_rx mem_rx))) ∗ *)
+  (*              (* rx pages for all other VMs *) *)
+  (*              rx_states_global (delete i rxs) ∗ ⌜is_total_gmap rxs⌝ ∗ *)
+  (*              (* if i yielding, we give following resources back to pvm *) *)
+  (*              VMProp V0 (vmprop_zero trans' rxs) (1/2)%Qp)%I. *)
+  (*   Proof. *)
+  (*     rewrite /vmprop_unknown. *)
+  (*     apply (fixpoint_unfold vmprop_unknown_pre). *)
+  (*   Qed. *)
+
+  Definition transferred_memory_slice (trans : gmap Addr transaction) (i: VMID) (j:VMID): iProp Σ:=
+    big_sepFM trans (λ kv, (kv.2.1.1.1.1 = i ∧ kv.2.1.1.1.2 = j) ∧ ¬(kv.2.2 = true ∧ kv.2.1.2 = Lending)) (λ _ tran, (∃ mem , memory_pages tran.1.1.2 mem)%I).
+
+  Definition retrievable_transaction_transferred_slice (trans : gmap Addr transaction) (i:VMID) (j: VMID) : iProp Σ :=
+    (big_sepFM trans (λ kv, kv.2.1.1.1.1 = i ∧ kv.2.1.1.1.2 = j) (λ k v, k -{1/2}>re v.2 )%I) ∗
+    (big_sepFM trans (λ kv, (kv.2.1.1.1.1 = i ∧ kv.2.1.1.1.2 = j) ∧ kv.2.2 = false) (λ k v, k -{1/4}>t v.1 ∗ k -{1/2}>re v.2)%I).
+
+  Definition transaction_pagetable_entries_transferred_slice (trans: gmap Addr transaction) (i: VMID) (j: VMID) : iProp Σ :=
+    big_sepFM trans (λ kv, (kv.2.1.1.1.1 = i ∧ kv.2.1.1.1.2 = j) ∧ kv.2.1.2 = Donation) (λ k v, k -{1/4}>t v.1 ∗ pgt_1_4 v.1.1.2 v.1.1.1.1 true)%I.
+
+  Definition slice_transfer_all :=
+    (λ trans i j, transaction_pagetable_entries_transferred_slice trans i j
+                ∗ retrievable_transaction_transferred_slice trans i j
+                ∗ transferred_memory_slice trans i j)%I.
+
+  Definition slice_rx_state (j : VMID) (os : option (Word * VMID)) : iProp Σ :=
+    (RX_state{1/2}@j := os) ∗ ∃ p_rx, RX@ j := p_rx ∗ (∃ mem_rx, memory_page p_rx mem_rx).
+
+  Definition interp_access p_tx p_rx ps_acc trans: iPropO Σ:=
     (
       (* exclusively owned pages are pages i has access to, but ain't in any transactions related to i. *)
       (* [ps_oea], we exclude all pages involved in in-flight transactions,
        NOTE: it has to be (currently_accessible_in_trans_memory_pages)*)
       let ps_oea := ps_acc ∖ {[p_rx;p_tx]} ∖ (currently_accessible_in_trans_memory_pages trans) in
+      ⌜∀ k j trans, (k = i ∨ j = i) -> Φ_t trans k j ⊣⊢ slice_transfer_all trans k j⌝ ∗
+      ⌜∀ os, (match os with
+                 | None => True
+                 | _ => Φ_r i os i ⊣⊢ slice_rx_state i os
+                end)⌝ ∗
+      ⌜∀ os, (match os with
+                 | None => True
+                 | _ => Φ_r i os V0 ⊣⊢ slice_rx_state i os
+                end)⌝ ∗
+      ⌜∀ k os, (match os with
+          | None => True
+          | Some (_, j) => j = i -> Φ_r k os V0 ⊣⊢ slice_rx_state k os
+          end)⌝ ∗
+      ⌜∀ i j, Φ_r i None j ⊣⊢ True⌝ ∗
       (* registers *)
       (∃ regs, ⌜is_total_gmap regs⌝ ∗ [∗ map] r ↦ w ∈ regs, r @@ i ->r w) ∗
       (* TX page and its memory *)
