theories/logrel/fundamental_prim.v
@@ -3,7 +3,7 @@ From machine_program_logic.program_logic Require Import weakestpre.
 From HypVeri.lang Require Import lang trans_extra.
 From HypVeri.algebra Require Import base pagetable mem trans mailbox.
 From HypVeri.rules Require Import rules_base halt fail run.
-From HypVeri.logrel Require Import logrel_prim_extra.
+From HypVeri.logrel Require Import logrel_prim logrel_prim_extra.
 From HypVeri.logrel Require Import ftlr_nop ftlr_mov ftlr_ldr ftlr_str ftlr_cmp ftlr_add ftlr_sub ftlr_mult ftlr_bne ftlr_br.
 From HypVeri.logrel Require Import ftlr_run_prim ftlr_yield_prim ftlr_share ftlr_retrieve ftlr_relinquish ftlr_reclaim ftlr_donate ftlr_lend
  ftlr_msg_wait_prim ftlr_msg_send_prim ftlr_msg_poll ftlr_invalid_hvc.
